<?xml version="1.0" encoding="utf-8"?>
<rdf:RDF
  xmlns:skos="http://www.w3.org/2004/02/skos/core#"
  xmlns:rdf="http://www.w3.org/1999/02/22-rdf-syntax-ns#"
  xmlns:ldp="http://www.w3.org/ns/ldp#"
  xmlns:owl="http://www.w3.org/2002/07/owl#"
  xmlns:rdfs="http://www.w3.org/2000/01/rdf-schema#"
  xmlns:reg="http://purl.org/linked-data/registry#"
  xmlns:dct="http://purl.org/dc/terms/"
>
  <reg:Register rdf:about="http://codes.wmo.int/common/nil">
    <skos:member>
      <skos:Concept rdf:about="http://codes.wmo.int/common/nil/AboveDetectionRange">
        <skos:notation>AboveDetectionRange</skos:notation>
        <rdfs:label xml:lang="en">Above detection range</rdfs:label>
        <dct:description xml:lang="en">The value was above the detection range of the instrument used to estimate it.</dct:description>
        <owl:versionInfo rdf:resource="http://icao.int/iwxxm/1.1"/>
        <owl:versionInfo rdf:resource="http://icao.int/iwxxm/2.1"/>
        <owl:versionInfo rdf:resource="http://icao.int/iwxxm/3.0"/>
        <owl:versionInfo rdf:resource="http://icao.int/iwxxm/2021-2"/>
        <owl:versionInfo rdf:resource="http://icao.int/iwxxm/2023-1"/>
        <owl:versionInfo rdf:resource="http://icao.int/iwxxm/2025-2"/>
      </skos:Concept>
    </skos:member>
    <skos:member>
      <skos:Concept rdf:about="http://codes.wmo.int/common/nil/BelowDetectionRange">
        <skos:notation>BelowDetectionRange</skos:notation>
        <rdfs:label xml:lang="en">Below detection range</rdfs:label>
        <dct:description xml:lang="en">The value was below the detection range of the instrument used to estimate it.</dct:description>
        <owl:versionInfo rdf:resource="http://icao.int/iwxxm/1.1"/>
        <owl:versionInfo rdf:resource="http://icao.int/iwxxm/2.1"/>
        <owl:versionInfo rdf:resource="http://icao.int/iwxxm/3.0"/>
        <owl:versionInfo rdf:resource="http://icao.int/iwxxm/2021-2"/>
        <owl:versionInfo rdf:resource="http://icao.int/iwxxm/2023-1"/>
        <owl:versionInfo rdf:resource="http://icao.int/iwxxm/2025-2"/>
      </skos:Concept>
    </skos:member>
    <skos:member>
      <skos:Concept rdf:about="http://codes.wmo.int/common/nil/inapplicable">
        <skos:notation>inapplicable</skos:notation>
        <rdfs:label xml:lang="en">Inapplicable</rdfs:label>
        <dct:description xml:lang="en">There is no value.</dct:description>
        <owl:versionInfo rdf:resource="http://icao.int/iwxxm/1.1"/>
        <owl:versionInfo rdf:resource="http://icao.int/iwxxm/2.1"/>
        <owl:versionInfo rdf:resource="http://icao.int/iwxxm/3.0"/>
        <owl:versionInfo rdf:resource="http://icao.int/iwxxm/2021-2"/>
        <owl:versionInfo rdf:resource="http://icao.int/iwxxm/2023-1"/>
        <owl:versionInfo rdf:resource="http://icao.int/iwxxm/2025-2"/>
      </skos:Concept>
    </skos:member>
    <skos:member>
      <skos:Concept rdf:about="http://codes.wmo.int/common/nil/missing">
        <skos:notation>missing</skos:notation>
        <rdfs:label xml:lang="en">Missing</rdfs:label>
        <dct:description xml:lang="en">The correct value is not readily available to the sender of this data. Furthermore, a correct value may not exist.</dct:description>
        <owl:versionInfo rdf:resource="http://icao.int/iwxxm/1.1"/>
        <owl:versionInfo rdf:resource="http://icao.int/iwxxm/2.1"/>
        <owl:versionInfo rdf:resource="http://icao.int/iwxxm/3.0"/>
        <owl:versionInfo rdf:resource="http://icao.int/iwxxm/2021-2"/>
        <owl:versionInfo rdf:resource="http://icao.int/iwxxm/2023-1"/>
        <owl:versionInfo rdf:resource="http://icao.int/iwxxm/2025-2"/>
      </skos:Concept>
    </skos:member>
    <skos:member>
      <skos:Concept rdf:about="http://codes.wmo.int/common/nil/noSignificantChange">
        <skos:notation>noSignificantChange</skos:notation>
        <rdfs:label xml:lang="en">No significant change</rdfs:label>
        <dct:description xml:lang="en">No significant change is expected to occur.</dct:description>
        <skos:altLabel xml:lang="en">NOSIG</skos:altLabel>
        <owl:versionInfo rdf:resource="http://icao.int/iwxxm/1.1"/>
        <owl:versionInfo rdf:resource="http://icao.int/iwxxm/2.1"/>
        <owl:versionInfo rdf:resource="http://icao.int/iwxxm/3.0"/>
        <owl:versionInfo rdf:resource="http://icao.int/iwxxm/2021-2"/>
        <owl:versionInfo rdf:resource="http://icao.int/iwxxm/2023-1"/>
        <owl:versionInfo rdf:resource="http://icao.int/iwxxm/2025-2"/>
      </skos:Concept>
    </skos:member>
    <skos:member>
      <skos:Concept rdf:about="http://codes.wmo.int/common/nil/notDetectedByAutoSystem">
        <skos:notation>notDetectedByAutoSystem</skos:notation>
        <rdfs:label xml:lang="en">Nothing detected by automated system</rdfs:label>
        <dct:description xml:lang="en">The automated observing system did not detect a value (e.g. no cloud detected NCD).</dct:description>
        <owl:versionInfo rdf:resource="http://icao.int/iwxxm/1.1"/>
        <owl:versionInfo rdf:resource="http://icao.int/iwxxm/2.1"/>
        <owl:versionInfo rdf:resource="http://icao.int/iwxxm/3.0"/>
        <owl:versionInfo rdf:resource="http://icao.int/iwxxm/2021-2"/>
        <owl:versionInfo rdf:resource="http://icao.int/iwxxm/2023-1"/>
        <owl:versionInfo rdf:resource="http://icao.int/iwxxm/2025-2"/>
      </skos:Concept>
    </skos:member>
    <skos:member>
      <skos:Concept rdf:about="http://codes.wmo.int/common/nil/notObservable">
        <skos:notation>notObservable</skos:notation>
        <rdfs:label xml:lang="en">Not observable</rdfs:label>
        <dct:description xml:lang="en">A system failure, sensor failure, or sensor obstruction, prevented the intended observation of the value.</dct:description>
        <owl:versionInfo rdf:resource="http://icao.int/iwxxm/1.1"/>
        <owl:versionInfo rdf:resource="http://icao.int/iwxxm/2.1"/>
        <owl:versionInfo rdf:resource="http://icao.int/iwxxm/3.0"/>
        <owl:versionInfo rdf:resource="http://icao.int/iwxxm/2021-2"/>
        <owl:versionInfo rdf:resource="http://icao.int/iwxxm/2023-1"/>
        <owl:versionInfo rdf:resource="http://icao.int/iwxxm/2025-2"/>
      </skos:Concept>
    </skos:member>
    <skos:member>
      <skos:Concept rdf:about="http://codes.wmo.int/common/nil/nothingOfOperationalSignificance">
        <skos:notation>nothingOfOperationalSignificance</skos:notation>
        <rdfs:label xml:lang="en">Nothing of operational signficance</rdfs:label>
        <dct:description xml:lang="en">Nothing was observed or forecast of operational significance (e.g. nil significant cloud NSC, nil significant weather NSW).</dct:description>
        <owl:versionInfo rdf:resource="http://icao.int/iwxxm/1.1"/>
        <owl:versionInfo rdf:resource="http://icao.int/iwxxm/2.1"/>
        <owl:versionInfo rdf:resource="http://icao.int/iwxxm/3.0"/>
        <owl:versionInfo rdf:resource="http://icao.int/iwxxm/2021-2"/>
        <owl:versionInfo rdf:resource="http://icao.int/iwxxm/2023-1"/>
        <owl:versionInfo rdf:resource="http://icao.int/iwxxm/2025-2"/>
      </skos:Concept>
    </skos:member>
    <skos:member>
      <skos:Concept rdf:about="http://codes.wmo.int/common/nil/template">
        <skos:notation>template</skos:notation>
        <rdfs:label xml:lang="en">Template</rdfs:label>
        <dct:description xml:lang="en">The value will be available later.</dct:description>
        <owl:versionInfo rdf:resource="http://icao.int/iwxxm/1.1"/>
        <owl:versionInfo rdf:resource="http://icao.int/iwxxm/2.1"/>
        <owl:versionInfo rdf:resource="http://icao.int/iwxxm/3.0"/>
        <owl:versionInfo rdf:resource="http://icao.int/iwxxm/2021-2"/>
        <owl:versionInfo rdf:resource="http://icao.int/iwxxm/2023-1"/>
        <owl:versionInfo rdf:resource="http://icao.int/iwxxm/2025-2"/>
      </skos:Concept>
    </skos:member>
    <skos:member>
      <skos:Concept rdf:about="http://codes.wmo.int/common/nil/unknown">
        <skos:notation>unknown</skos:notation>
        <rdfs:label xml:lang="en">Unknown</rdfs:label>
        <dct:description xml:lang="en">The correct value is not known to, and not computable by, the sender of this data. However, a correct value probably exists.</dct:description>
        <owl:versionInfo rdf:resource="http://icao.int/iwxxm/1.1"/>
        <owl:versionInfo rdf:resource="http://icao.int/iwxxm/2.1"/>
        <owl:versionInfo rdf:resource="http://icao.int/iwxxm/3.0"/>
        <owl:versionInfo rdf:resource="http://icao.int/iwxxm/2021-2"/>
        <owl:versionInfo rdf:resource="http://icao.int/iwxxm/2023-1"/>
        <owl:versionInfo rdf:resource="http://icao.int/iwxxm/2025-2"/>
      </skos:Concept>
    </skos:member>
    <skos:member>
      <skos:Concept rdf:about="http://codes.wmo.int/common/nil/withheld">
        <skos:notation>withheld</skos:notation>
        <rdfs:label xml:lang="en">Withheld</rdfs:label>
        <dct:description xml:lang="en">The value is not divulged.</dct:description>
        <owl:versionInfo rdf:resource="http://icao.int/iwxxm/1.1"/>
        <owl:versionInfo rdf:resource="http://icao.int/iwxxm/2.1"/>
        <owl:versionInfo rdf:resource="http://icao.int/iwxxm/3.0"/>
        <owl:versionInfo rdf:resource="http://icao.int/iwxxm/2021-2"/>
        <owl:versionInfo rdf:resource="http://icao.int/iwxxm/2023-1"/>
        <owl:versionInfo rdf:resource="http://icao.int/iwxxm/2025-2"/>
      </skos:Concept>
    </skos:member>
    <rdf:type rdf:resource="http://www.w3.org/ns/ldp#Container"/>
    <rdf:type rdf:resource="http://www.w3.org/2004/02/skos/core#Collection"/>
    <skos:notation>nil</skos:notation>
    <rdfs:label xml:lang="en">Code Table D-1: Nil reasons</rdfs:label>
    <dct:description xml:lang="en">Nil-reason terms are used to provide an explanation for recording a missing (or void) value within a data product. Terms are drawn from authorities in addition to WMO including ISO/TC 211 (from ISO 19136:2007 Geography markup language clause 8.2.3.1; published on their behalf by the Open Geospatial Consortium).</dct:description>
    <owl:versionInfo rdf:resource="http://icao.int/iwxxm/1.1"/>
    <owl:versionInfo rdf:resource="http://icao.int/iwxxm/2.1"/>
    <owl:versionInfo rdf:resource="http://icao.int/iwxxm/3.0"/>
    <owl:versionInfo rdf:resource="http://icao.int/iwxxm/2021-2"/>
    <owl:versionInfo rdf:resource="http://icao.int/iwxxm/2023-1"/>
    <owl:versionInfo rdf:resource="http://icao.int/iwxxm/2025-2"/>
    <ldp:hasMemberRelation rdf:resource="http://www.w3.org/2004/02/skos/core#member"/>
  </reg:Register>
</rdf:RDF>
